

Let \underline{w} denote the state. A general form of governing equation is assumed to be

$$\underline{r} = \underline{f}(\underline{w}) - \underline{h}(\dot{\underline{w}}) - \underline{g}(\ddot{\underline{w}})$$

The discrete form is assumed to be

$$\underline{r}^n = \underline{f}(\underline{w}^n; \underline{w}^{n-1}) - \underline{h}(\dot{\underline{w}}^n; \dot{\underline{w}}^{n-1}) - \underline{g}(\ddot{\underline{w}}^n; \ddot{\underline{w}}^{n-1})$$

Here $\underline{f}^n, \underline{h}^n, \underline{g}^n$ only depend on $\underline{w}^{n-1}, \dot{\underline{w}}^{n-1}, \ddot{\underline{w}}^{n-1}$ if the time discretization is based on intermediate states $\underline{w}^{n-\alpha}, \dot{\underline{w}}^{n-\beta}, \ddot{\underline{w}}^{n-\gamma}$.

Lagrangian:

$$L = \sum_{k=1}^N [J^k + \underline{\lambda}^{kT} \underline{r}^k + \underline{\lambda}_1^{kT} \underline{c}_1^k + \underline{\lambda}_2^{kT} \underline{c}_2^k] \quad (\underline{c}_1 \text{ and } \underline{c}_2 \text{ are defined by time discretization})$$

Adjoint equations at step 'n':

$$\frac{\partial L}{\partial \underline{w}^n} = \frac{\partial J^n}{\partial \underline{w}^n} + \frac{\partial J^{n+1}}{\partial \underline{w}^n} + \underline{\lambda}^{nT} \frac{\partial \underline{r}^n}{\partial \underline{w}^n} + \underline{\lambda}^{n+1T} \frac{\partial \underline{r}^{n+1}}{\partial \underline{w}^n} + \underline{\lambda}_1^{nT} \frac{\partial \underline{c}_1^n}{\partial \underline{w}^n} + \underline{\lambda}_1^{n+1T} \frac{\partial \underline{c}_1^{n+1}}{\partial \underline{w}^n} + \dots = 0$$

$$\frac{\partial L}{\partial \dot{\underline{w}}^n} = \frac{\partial J^n}{\partial \dot{\underline{w}}^n} + \frac{\partial J^{n+1}}{\partial \dot{\underline{w}}^n} + \underline{\lambda}^{nT} \frac{\partial \underline{r}^n}{\partial \dot{\underline{w}}^n} + \underline{\lambda}^{n+1T} \frac{\partial \underline{r}^{n+1}}{\partial \dot{\underline{w}}^n} + \underline{\lambda}_1^{nT} \frac{\partial \underline{c}_1^n}{\partial \dot{\underline{w}}^n} + \underline{\lambda}_1^{n+1T} \frac{\partial \underline{c}_1^{n+1}}{\partial \dot{\underline{w}}^n} + \dots = 0$$

$$\frac{\partial L}{\partial \ddot{\underline{w}}^n} = \frac{\partial J^n}{\partial \ddot{\underline{w}}^n} + \frac{\partial J^{n+1}}{\partial \ddot{\underline{w}}^n} + \underline{\lambda}^{nT} \frac{\partial \underline{r}^n}{\partial \ddot{\underline{w}}^n} + \underline{\lambda}^{n+1T} \frac{\partial \underline{r}^{n+1}}{\partial \ddot{\underline{w}}^n} + \dots = 0$$

The element needs to provide $\frac{\partial \underline{r}^{(n+1)}}{\partial \underline{w}^n}, \frac{\partial \underline{r}^{(n+1)}}{\partial \dot{\underline{w}}^n}, \frac{\partial \underline{r}^{(n+1)}}{\partial \ddot{\underline{w}}^n}$. The objective function provides the terms containing J and the scheme builds the system at the element level including contributions from \underline{c}_1 and \underline{c}_2 .

Example:

The VMS element doesn't conform to the above governing equation since stabilization introduces velocity into mass matrix and $\underline{g}^n = \underline{g}^n(\dot{\underline{w}}^n, \ddot{\underline{w}}^n; \dot{\underline{w}}^{n-1})$.

$$\underline{r}^n = -\underline{D}(\dot{\underline{w}}^n) \dot{\underline{w}}^{n+\alpha-1} - \underline{M}(\dot{\underline{w}}^n) \ddot{\underline{w}}^{n+\alpha-1} = -\underline{h}(\dot{\underline{w}}^n; \dot{\underline{w}}^{n-1}) - \underline{g}(\dot{\underline{w}}^n, \ddot{\underline{w}}^n; \dot{\underline{w}}^{n-1})$$

$$L = \sum_{k=1}^N [J^k + \underline{\lambda}^{kT} (\alpha_f \underline{h}^k + (1-\alpha_f) \underline{h}^{k-1} + \alpha_m \underline{M}^k \ddot{\underline{w}}^k + (1-\alpha_m) \underline{M}^{k-1} \ddot{\underline{w}}^{k-1}) + \underline{\lambda}_2^{kT} (\ddot{\underline{w}}^{k-1} - \frac{\gamma}{(r-1)} \ddot{\underline{w}}^k + \frac{\dot{\underline{w}}^k - \dot{\underline{w}}^{k-1}}{(r-1)\Delta t})]$$

$$\frac{\partial L}{\partial \underline{w}^n} = \frac{1}{(r-1)\Delta t} (\underline{\lambda}_2^n - \underline{\lambda}_2^{n+1}) + \partial \dot{\underline{w}}^n \underline{h}^{nT} [\alpha_f \underline{\lambda}^n + (1-\alpha_f) \underline{\lambda}^{n+1}] + \partial \dot{\underline{w}}^n \{ \underline{M}^n \ddot{\underline{w}}^{n+\alpha-1} \}^T \underline{\lambda}^n = -\frac{\partial J^n}{\partial \underline{w}^n} - \frac{\partial J^{n+1}}{\partial \underline{w}^n}$$

$$\frac{\partial L}{\partial \dot{\underline{w}}^n} = -\frac{\gamma}{(r-1)} \underline{\lambda}_2^n + \underline{\lambda}_2^{n+1} + \underbrace{\alpha_m \underline{M}^{nT}}_{\partial \dot{\underline{w}}^n \underline{g}^n} \underline{\lambda}^n + \underbrace{(1-\alpha_m) \underline{M}^{nT}}_{\partial \dot{\underline{w}}^n \underline{g}^{n+1}} \underline{\lambda}^{n+1} = -\frac{\partial J^n}{\partial \dot{\underline{w}}^n} - \frac{\partial \dot{\underline{w}}^n \underline{g}^{nT}}{\partial \dot{\underline{w}}^n}$$

If $\alpha_f \neq 1$ we need element functions to get $\partial \dot{\underline{w}}^n \underline{h}^{nT}$ and $\partial \dot{\underline{w}}^n \{ \underline{M}^n \ddot{\underline{w}}^{n+\alpha-1} \}^T$ separately to combine in the scheme (we want it to be possible to keep element and time discretization separate). But, the element function which provides $\partial \underline{r}^{(n+1)} / \partial \dot{\underline{w}}^n = -\partial \dot{\underline{w}}^n \underline{h}^{nT} - \partial \dot{\underline{w}}^n \{ \underline{M}^n \ddot{\underline{w}}^{n+\alpha-1} \}^T$ doesn't do this. This is an exceptional case of the VMS formulation which makes \underline{g}^n dependent on $\dot{\underline{w}}^n$. If we restrict to Bassak ($\alpha_f = 1$) then it is not a problem. Also the element does not need to know α_m to calculate $\ddot{\underline{w}}^{n+\alpha-1}$ since the acceleration is already saved in this format during primal solution.

We can eliminate the 'order' parameter, which is confusing, if we define separate functions:

$$\text{Element}::\text{AdjointMatrix}(\text{not step}=0) \mapsto \frac{\partial \underline{r}^{(n+1)T}}{\partial \underline{w}^n} = \frac{\partial \underline{f}^{(n+1)T}}{\partial \underline{w}^n}$$

$$\text{Element}::\text{AdjointDampingMatrix}(\text{not step}=0) \mapsto -\frac{\partial \underline{r}^{(n+1)T}}{\partial \dot{\underline{w}}^n} = \frac{\partial \underline{h}^{(n+1)T}}{\partial \dot{\underline{w}}^n}$$

$$\text{Element}::\text{AdjointMassMatrix}(\text{not step}=0) \mapsto -\frac{\partial \underline{r}^{(n+1)T}}{\partial \ddot{\underline{w}}^n} = \frac{\partial \underline{g}^{(n+1)T}}{\partial \ddot{\underline{w}}^n}$$